FallDecoupled.v
@@ -1,0 +1,254 @@
+Require Import FlowEquivalence.
+Require Import List.
+Import ListNotations.
+Open Scope list_scope.
+
+
+
+Require Import PeanoNat.
+Infix "<?" := (Nat.ltb).
+
+Existing Instance event_eq_dec.
+Existing Instance latch_eq_dec.
+
+Require Import Coq.Logic.FunctionalExtensionality.
+Import Coq.Logic.ProofIrrelevance.
+
+
+Section FallDecoupled.
+
+  Context (even odd : Set).
+  Context `{Heven : eq_dec even} `{Hodd : eq_dec odd}.
+  Variable c : circuit even odd.
+  Variable init_st : state (latch even odd).
+
+
+  Inductive transitions_FD : Set :=
+  | Even_fall (A : even) : transitions_FD
+  | Even_rise (A : even) : transitions_FD
+  | Odd_fall  (B : odd) : transitions_FD
+  | Odd_rise  (B : odd) : transitions_FD
+  | Even_rise_odd_rise (E : even) (O : odd) : In (E,O) (even_odd_neighbors c) -> transitions_FD (* E+ → O+ *)
+  | Odd_fall_even_rise (E : even) (O : odd) : In (E,O) (even_odd_neighbors c) -> transitions_FD (* O- → E+ *)
+  | Odd_rise_even_rise (O : odd) (E : even) : In (O,E) (odd_even_neighbors c) -> transitions_FD (* O+ → E+ *)
+  | Even_fall_odd_rise (O : odd) (E : even) : In (O,E) (odd_even_neighbors c) -> transitions_FD (* E- → O+ *)
+  .
+  Instance eqdecFD : eq_dec transitions_FD.
+  Proof.
+    split. intros t1 t2.
+    destruct Heven as [Heven'], Hodd as [Hodd'].
+    destruct t1; destruct t2; try (right; inversion 1; fail);
+      try (destruct (Dec A A0) as [HA | HA];
+        [subst; intuition | right; inversion 1; contradiction]);
+      try (destruct (Dec B B0) as [HB | HB];
+        [subst; intuition | right; inversion 1; contradiction]).
+  Admitted.
+
+  Definition fall_decoupled 
+           : marked_graph (event even odd) transitions_FD :=
+  {| mg_triples := 
+     let eo_f := fun (E : even) (O : odd) pf =>
+                     [ (Rise (Even E), Even_fall E, Fall (Even E))
+                     ; (Fall (Even E), Even_rise E, Rise (Even E))
+                     ; (Rise (Even E), Even_rise_odd_rise E O pf, Rise (Odd O))
+                     ; (Fall (Odd O), Odd_fall_even_rise E O pf, Rise (Even E))
+                     ; (Rise (Odd O), Odd_fall O, Fall (Odd O))
+                     ]
+     in
+     let oe_f := fun (O : odd) (E : even) pf =>
+                     [ (Rise (Odd O), Odd_fall O, Fall (Odd O))
+                     ; (Fall (Odd O), Odd_rise O, Rise (Odd O))
+                     ; (Rise (Odd O), Odd_rise_even_rise O E pf, Rise (Even E))
+                     ; (Fall (Even E), Even_fall_odd_rise O E pf, Rise (Odd O))
+                     ; (Rise (Even E), Even_fall E, Fall (Even E))
+                     ]
+     in flat_map_proof (even_odd_neighbors c) eo_f
+     ++ flat_map_proof (odd_even_neighbors c) oe_f
+   ; mg_init := fun p => match p with
+                | Even_rise_odd_rise _ _ _ => 1
+                | Even_fall _ => 1
+                | Odd_rise _ => 1
+                | _ => 0
+                end
+   |}.
+
+
+
+  Lemma event_rise_invariant_fd : forall t m st st' l,
+    {fall_decoupled}⊢ t ↓ m ->
+    c ⊢ init_st ⇒t⇒ st ->
+    async_step c (transparent t) st (Rise l) st' ->
+    forall l', l' <> l -> st'(l') = st(l').
+  Admitted.
+
+  Lemma event_invariant_neq : forall t m st st' e,
+    {fall_decoupled}⊢ t ↓ m ->
+    c ⊢ init_st ⇒t⇒ st ->
+    async_step c (transparent t) st e st' ->
+    forall l, e <> Rise l -> st'(l) = st(l).
+  Proof.
+    intros t m st st' e Hm Hst Hstep l Hl.
+    destruct e as [l' | l'].
+    * eapply event_rise_invariant_fd; eauto.
+      inversion 1; subst; contradiction.
+    * eapply event_fall_invariant; eauto.
+  Qed.
+
+
+
+Lemma rise_enabled_even_odd : forall t m O E,
+    {fall_decoupled}⊢ t ↓ m ->
+    is_enabled fall_decoupled (Rise (Odd O)) m ->
+    In (E,O) (even_odd_neighbors c) ->
+    num_events (Rise (Even E)) t = num_events (Rise (Odd O)) t.
+Admitted.
+
+Lemma rise_enabled_odd_even : forall t m O E,
+    {fall_decoupled}⊢ t ↓ m ->
+    is_enabled fall_decoupled (Rise (Even E)) m ->
+    In (O,E) (odd_even_neighbors c) ->
+    num_events (Rise (Odd O)) t = 1+num_events (Rise (Even E)) t.
+Admitted.
+
+  Lemma fall_decoupled_strong : 
+    forall t,
+      forall m, {fall_decoupled}⊢ t ↓ m ->
+      forall st, c ⊢ init_st ⇒t⇒ st ->
+      (forall O, st(Odd O) = sync_eval c init_st (num_events (Rise (Odd O)) t) (Odd O)) /\
+      (forall E, st(Even E) = sync_eval c init_st (1+num_events (Rise (Even E)) t) (Even E)).
+  Proof.
+    induction t as [P | e t];
+      intros m Hm st Heval;
+      split; intros l.
+    * (* base case, odd *)
+      simpl. inversion Heval; subst. rewrite sync_eval_odd_0. reflexivity.
+    * (* base case, even *)
+      simpl. inversion Heval; subst.
+      erewrite eval_transparent; eauto.
+      { simpl. rewrite sync_eval_even.
+        f_equal.
+        unfold odd_state.
+        apply functional_extensionality.
+        intros [O Ho]. simpl.
+        rewrite sync_eval_odd_0. reflexivity.
+      }
+      { simpl.
+        inversion Hm as [P0 Hopaque Htransparent | ]; clear H P0; rewrite <- H2 in *; clear m H2.
+        apply Htransparent.
+
+        (* apply is_enabled_fd. *)
+        admit (* LEMMA *).
+      }
+    * (* inductive case, odd *)
+
+      inversion Hm as [ | e0' m0 m0' s' Henabled Hfire Hconsistent']; subst;
+        rename m0 into m.
+      inversion Heval as [ | ? ? st' ? Heval' Hopaque' Htransparent']; subst.
+      simpl in *.
+
+      destruct (Dec (Rise (Odd l)) e).
+      (* If e = l+, then l is transparent in (e::t) *)
+      { subst. rewrite eqb_eq.
+        rewrite Htransparent'.
+        2:{ unfold update_transparency_predicate. rewrite eqb_eq. auto. }
+        simpl.
+        rewrite sync_eval_odd.
+        
+        f_equal. apply functional_extensionality. 
+        unfold even_state. intros [E He].
+        simpl.
+
+        rewrite (event_rise_invariant_fd t m st' st (Odd l)); auto.
+        2:{ split; auto. }
+        2:{ inversion 1. }
+
+        destruct (IHt m Hconsistent' st' Heval') as [_ IH].
+        rewrite IH.
+        
+        assert (Hnum : num_events (Rise (Even E)) t = num_events (Rise (Odd l)) t).
+        { eapply rise_enabled_even_odd; eauto.  }
+
+        rewrite Hnum. reflexivity.
+      }
+
+      rewrite eqb_neq; auto.
+    
+
+      rewrite (event_invariant_neq t m st' st e); eauto.
+      2:{ split; auto. }
+
+      destruct (IHt m Hconsistent' st' Heval') as [IH _].
+      rewrite IH.
+      reflexivity.
+      
+      
+
+    * (* inductive case, even *)
+      inversion Hm as [ | e0' m0 m0' s' Henabled Hfire Hconsistent']; subst;
+        rename m0 into m.
+      inversion Heval as [ | ? ? st' ? Heval' Hopaque' Htransparent']; subst.
+      simpl in *.
+
+      destruct (Dec (Rise (Even l)) e).
+      (* If e = l+, then l is transparent in (e::t) *)
+      { subst. rewrite eqb_eq.
+        rewrite Htransparent'.
+        2:{ unfold update_transparency_predicate. rewrite eqb_eq. auto. }
+        simpl.
+        rewrite sync_eval_even.
+        
+        f_equal. apply functional_extensionality. 
+        unfold odd_state. intros [O He].
+        simpl.
+
+        rewrite (event_rise_invariant_fd t m st' st (Even l)); auto.
+        2:{ split; auto. }
+        2:{ inversion 1. }
+
+        destruct (IHt m Hconsistent' st' Heval') as [IH _].
+        rewrite IH.
+        
+        assert (Hnum : num_events (Rise (Odd O)) t = 1+num_events (Rise (Even l)) t).
+        { eapply rise_enabled_odd_even; eauto. }
+
+        rewrite Hnum. reflexivity.
+      }
+
+      rewrite eqb_neq; auto.
+    
+      rewrite (event_invariant_neq t m st' st e); eauto.
+      2:{ split; auto. }
+      destruct (IHt m Hconsistent' st' Heval') as [_ IH].
+      rewrite IH.
+      reflexivity.
+  Admitted.
+      
+
+Lemma num_events_odd_opaque : forall t st m O,
+    c ⊢ init_st ⇒t⇒ st ->
+    {fall_decoupled}⊢ t ↓ m ->
+    transparent t (Odd O) = false ->
+    num_events (Rise (Odd O)) t = num_events (Fall (Odd O)) t.
+Admitted.
+Lemma num_events_even_opaque : forall t st m E,
+    c ⊢ init_st ⇒t⇒ st ->
+    {fall_decoupled}⊢ t ↓ m ->
+    transparent t (Even E) = false ->
+    num_events (Fall (Even E)) t = 1 + num_events (Rise (Even E)) t.
+Admitted. 
+
+        
+  Theorem fall_decoupled_flow_equivalence :
+    flow_equivalence fall_decoupled c init_st.
+  Proof.
+    intros t [m Hm] st Hst l Hopaque.
+    destruct (fall_decoupled_strong t m Hm st Hst) as [HO HE].
+    destruct l as [O | E].
+    + rewrite HO.
+      erewrite num_events_odd_opaque; eauto.
+    + rewrite HE.
+      erewrite num_events_even_opaque; eauto.
+  Qed.
+
+
+End FallDecoupled.
